Native word lib, corrected signed semantics, using records for programs, proc_table->syntactic program, execute-function

src/Com.thy
@@ -4,7 +4,7 @@ begin
 
 type_synonym fname = string
 
-datatype_new
+datatype
   com = SKIP
       | Assignl lexp exp       ("_ ::== _" [1000, 61] 61)
       | Assign  vname exp      ("_ ::= _" [1000, 61] 61)
@@ -19,26 +19,75 @@ datatype_new
 term "''x'' ::= ''fun'' ([])"
 term "(Derefl (V ''x'')) ::== ''fun'' ([])"
 
-type_synonym fun_decl = "vname list \<times> vname list \<times> com"
+record fun_decl =
+  name :: fname
+  params :: "vname list"
+  locals :: "vname list"
+  body :: com
 
-fun def_returns :: "com \<Rightarrow> bool" where
+hide_const (open) name params locals body
+
+(*fun def_returns :: "com \<Rightarrow> bool" where
   "def_returns (Return _) \<longleftrightarrow> True"
 | "def_returns (c1 ;; c2) \<longleftrightarrow> def_returns c1 \<or> def_returns c2"
 | "def_returns (IF _ THEN c1 ELSE c2) \<longleftrightarrow> def_returns c1 \<and> def_returns c2"
 | "def_returns _ \<longleftrightarrow> False"
+*)
 
 fun valid_fun_decl :: "fun_decl \<Rightarrow> bool" 
-  where "valid_fun_decl (params,locals,com) \<longleftrightarrow> 
-    distinct (params @ locals)
-  \<and> def_returns com"
+  where "valid_fun_decl fdecl \<longleftrightarrow> 
+    distinct (fun_decl.params fdecl @ fun_decl.locals fdecl)"
 
-type_synonym program = "fname \<Rightarrow> fun_decl option"
+type_synonym global_decl = string
+
+record program =
+  globals :: "vname list"
+  procs :: "fun_decl list"
+
+hide_const (open) globals procs
+
+type_synonym proc_table = "fname \<rightharpoonup> fun_decl"
+
+definition proc_table_of :: "program \<Rightarrow> proc_table" where
+  "proc_table_of p = map_of (map (\<lambda>fd. (fun_decl.name fd, fd)) (program.procs p))"
 
 definition valid_program :: "program \<Rightarrow> bool" 
-  where "valid_program p \<equiv> (\<forall>fd\<in>ran p. valid_fun_decl fd)
-    \<and> ''main'' \<in> dom p
-    \<and> fst (the (p ''main'')) = []"
+  where "valid_program p \<equiv> 
+      distinct (program.globals p)
+    \<and> distinct (map fun_decl.name (program.procs p))
+    \<and> (\<forall>fd\<in>set (program.procs p). valid_fun_decl fd)
+    \<and> ( let
+          pt = proc_table_of p
+        in
+         ''main'' \<in> dom pt
+       \<and> fun_decl.params (the (pt ''main'')) = []
+      )"
 
+context begin
+
+private lemma dom_pt_of_alt: "dom (proc_table_of p) = set (map fun_decl.name (program.procs p))"
+  unfolding proc_table_of_def 
+  apply (simp add: dom_map_of_conv_image_fst)
+  apply force
+  done
+
+lemma valid_program_code[code]: "valid_program p \<longleftrightarrow>
+      distinct (program.globals p)
+    \<and> distinct (map fun_decl.name (program.procs p))
+    \<and> (\<forall>fd\<in>set (program.procs p). valid_fun_decl fd)
+    \<and> ''main'' \<in> set (map fun_decl.name (program.procs p))
+    \<and> (let
+          pt = proc_table_of p
+       in
+         fun_decl.params (the (pt ''main'')) = []
+      )"
+  unfolding valid_program_def
+  unfolding Let_def
+  apply (subst dom_pt_of_alt)
+  by simp
+    
+    
+end
 
 end
 
